Added alternative sequential version of bloom filter

theories/coneris/examples/bloom_filter/concurrent_bloom_filter_alt.v
@@ -52,6 +52,22 @@ Section conc_bloom_filter.
       lookup_bloom_filter "bfl" ktest.
 
 
+  Definition insert_bloom_filter_loop_seq : val :=
+    (rec: "aux" "bfl" "ks" :=
+       match: "ks" with
+         NONE => #()
+       | SOME "p" =>
+           let: "h" := Fst "p" in
+           let: "t" := Snd "p" in
+           (insert_bloom_filter "bfl" "h") ;; ("aux" "bfl" "t")
+       end).
+
+  Definition main_bloom_filter_seq (ksv ktest : val) : expr :=
+      let: "bfl" := init_bloom_filter #() in
+      insert_bloom_filter_loop_seq "bfl" ksv ;;
+      lookup_bloom_filter "bfl" ktest.
+
+
   Definition con_hash_inv_list hfs hnames ks (s : gset nat) :=
     ([∗ list] i ↦f;γ ∈ hfs;hnames,
        conhashfun γ filter_size f ∗
@@ -583,22 +599,58 @@ Section conc_bloom_filter.
         by iApply "HΦ".
   Qed.
 
- Lemma main_bloom_filter_spec (N : namespace) (ks : list nat) (ksv : val) (ktest : nat) :
+
+  Lemma insert_bloom_filter_loop_seq_spec N bfl hfuns a hnames s
+          (ns ks : list nat) (ksv : val) :
+    is_list ks ksv ->
+    {{{ bloom_filter_inv N bfl hfuns a hnames ns s ∗
+        ([∗ list] k ∈ ks, ⌜k ∈ ns ⌝) ∗
+        ([∗ list] k ∈ ns, ⌜ (k ≤ max_key)%nat ⌝)
+    }}}
+      insert_bloom_filter_loop_seq #bfl ksv
+    {{{ v, RET v; True }}}.
+  Proof.
+    iIntros (Hksv Φ) "(#Hinv & %Hks & %Hns) HΦ".
+    rewrite /insert_bloom_filter_loop_seq.
+    iInduction ks as [|k ks'] "IH" forall (ksv Hksv Φ).
+    - simpl in Hksv.
+      simplify_eq.
+      wp_pures.
+      by iApply "HΦ".
+    - destruct Hksv as [kv [-> Htail]].
+      wp_pures.
+      simpl.
+      wp_bind (insert_bloom_filter _ _).
+      wp_apply (bloom_filter_insert_thread_spec _ _ _ _ _ _ ns); auto.
+      { apply (Hks 0); auto. }
+      iIntros "_".
+      do 2 wp_pure.
+      iSpecialize ("IH" with "[]").
+      {
+        iPureIntro.
+        intros i ? ?.
+        apply (Hks (S i)).
+        auto.
+      }
+      iApply "IH"; auto.
+  Qed.
+
+ Lemma main_bloom_filter_seq_spec (N : namespace) (ks : list nat) (ksv : val) (ktest : nat) :
       NoDup ks ->
       is_list ks ksv ->
       ktest ∉ ks ->
       (ktest ≤ max_key)%nat ->
       {{{ ([∗ list] k ∈ ks, ⌜ (k ≤ max_key)%nat ⌝) ∗
            ↯ (fp_error filter_size num_hash (num_hash * length ks) 0) }}}
-        main_bloom_filter ksv #ktest
+        main_bloom_filter_seq ksv #ktest
       {{{ v, RET v; ⌜ v = #false ⌝ }}}.
  Proof.
    iIntros (Hndup Hksv Hktest Htestvalid Φ) "(#Hks & Herr) HΦ".
-   rewrite /main_bloom_filter.
+   rewrite /main_bloom_filter_seq.
    wp_apply (bloom_filter_init_spec N ks with "[//] Herr"); auto.
    iIntros (bfl) "(%hfuns & %a & %hnames & %s & Herr & Hauths & #Hinv)".
    wp_pures.
-   wp_apply (insert_bloom_filter_loop_spec N _ _ _ _ _ ks ks); auto.
+   wp_apply (insert_bloom_filter_loop_seq_spec N _ _ _ _ _ ks ks); auto.
    {
      repeat iSplit; auto.
      iPureIntro.
